theories/approxis/examples/prf.v
@@ -2,34 +2,142 @@ From clutch.approxis Require Import approxis map list security_aux option.
 From clutch.approxis Require Export bounded_oracle.
 Set Default Proof Using "Type*".
 
+(* Right-associative tuples. Alas, this breaks Coq's built-in tuple notation. *)
+(* Notation "( e1 ; e2 )" := (Pair e1 e2) : expr_scope.
+   Notation "( e1 ; e2 ; .. ; en' ; en )" := (Pair e1 (Pair e2 .. (Pair en' en) ..)) : expr_scope.
+   Notation "( e1 ; e2 )" := (PairV e1 e2) : val_scope.
+   Notation "( e1 ; e2 ; .. ; en' ; en )" := (PairV e1 (PairV e2 .. (PairV en' en) ..)) : val_scope. *)
 
-(* rand_output is currently unused ; it would be useful if a PRF module had
-   abstract types. *)
-Class PRF :=
+Class PRF_params :=
   { card_key : nat
   ; card_input : nat
   ; card_output : nat
-  ; keygen : val
+  ; prf_params : val := (#card_key, #card_input, #card_output) }.
+
+Definition get_param_card_key : val := λ:"prf_params", Fst (Fst "prf_params").
+Definition get_param_card_input : val := λ:"prf_params", Snd (Fst "prf_params").
+Definition get_param_card_output : val := λ:"prf_params", Snd "prf_params".
+
+(* rand_output is currently unused ; it would be useful if a PRF module had
+   abstract types. *)
+Class PRF `{PRF_params} :=
+  { keygen : val
   ; prf : val
   ; rand_output : val
+  ; prf_scheme : val := (prf_params, keygen, prf, rand_output)%V
   }.
 
+Definition get_params : val := λ:"prf_scheme", Fst (Fst (Fst "prf_scheme")).
+Definition get_card_key : val := λ:"prf_scheme", Fst (Fst (Fst (Fst (Fst "prf_scheme")))).
+Definition get_card_input : val := λ:"prf_scheme", Snd (Fst (Fst (Fst (Fst "prf_scheme")))).
+Definition get_card_output : val := λ:"prf_scheme", Snd (Fst (Fst (Fst "prf_scheme"))).
+Definition get_keygen : val := λ:"prf_scheme", Snd (Fst (Fst "prf_scheme")).
+Definition get_prf : val := λ:"prf_scheme", Snd (Fst ("prf_scheme")).
+Definition get_rand_output : val := λ:"prf_scheme", Snd "prf_scheme".
+
+
 (* An idealised random function family. *)
-Definition random_function (card_output : nat) : val :=
-  λ: "_key",
+Definition random_function : val :=
+  λ: "card_output",
     (* Create a reference to a functional map *)
     let: "mapref" := init_map #() in
     λ: "x",
       match: get "mapref" "x" with
       | SOME "y" => "y"
       | NONE =>
-          let: "y" := (rand #card_output) in
+          let: "y" := (rand "card_output") in
           set "mapref" "x" "y";;
           "y"
       end.
 
-Section lrel.
-  Context `{PRF}.
+(** PRF security definitions using the variant of q_calls with explicit bounds
+    checks in the code. **)
+Module bounds_check.
+  Section bounds_check.
+
+    (* Context `{PRF_scheme : PRF}. *)
+
+    (* Variable Key Input Output : nat.
+
+     Let keygen PRF_scheme : expr := Fst PRF_scheme.
+     Let prf PRF_scheme : expr := Fst (Snd PRF_scheme).
+     Let rand_output PRF_scheme : expr := Snd (Snd PRF_scheme). *)
+
+    (* Let q_calls := q_calls (card_input PRF_scheme). *)
+
+    Definition PRF_real_rand : val :=
+      λ:"b" "adv" "PRF_scheme" "Q",
+        let: "key" := get_keygen "PRF_scheme" #() in
+        let: "prf_key_b" :=
+          if: "b" then
+            get_prf "PRF_scheme" "key"
+          else
+            random_function (get_card_output "PRF_scheme") in
+        let: "oracle" := q_calls (get_card_input "PRF_scheme") "Q" "prf_key_b" in
+        let: "b'" := "adv" "oracle" in
+        "b'".
+
+    Definition wPRF : val :=
+      λ:"b" "PRF_scheme" "Q",
+        let: "key" := get_keygen "PRF_scheme" #() in
+        let: "prf_key_b" :=
+          if: "b" then
+            get_prf "PRF_scheme" "key"
+          else
+            random_function (get_card_output "PRF_scheme") in
+        let: "res" := ref list_nil in
+        letrec: "loop" "i" :=
+        if: "i" = #0 then #() else
+          let: "x" := rand (get_card_input "PRF_scheme") in
+          let: "y" := "prf_key_b" "x" in
+          "res" <- list_cons ("x", "y") (!"res") ;;
+          "loop" ("i" - #1)
+            in
+            ("loop" "Q") ;;
+            ! "res".
+
+    (* Rosulek, Def. 6.1 (PRF security) *)
+    (* NB: Rosulek samples the key from {0,1}^λ, we sample it from [0,card_key]. *)
+    Definition PRF_real : val :=
+      λ:"PRF_scheme" "Q",
+        let: "k" := get_keygen "PRF_scheme" #() in
+        let: "lookup" := get_prf "PRF_scheme" "k" in
+        let: "oracle" := q_calls (get_card_input "PRF_scheme") "Q" "lookup" in
+        "oracle".
+
+    Definition PRF_rand : val :=
+      λ:"PRF_scheme" "Q",
+        let: "lookup" := random_function (get_card_output "PRF_scheme") in
+        let: "oracle" := q_calls (get_card_input "PRF_scheme") "Q" "lookup" in
+        "oracle".
+
+  End bounds_check.
+End bounds_check.
+
+Module sem.
+  (** PRF security definitions using the variant of q_calls using semantic typing
+    instead of bounds checks. **)
+  Section sem.
+
+    Definition PRF_real : val :=
+      λ:"PRF" "Q",
+        let: "k" := get_keygen "PRF" #() in
+        let: "lookup" := get_prf "PRF" "k" in
+        let: "oracle" := q_calls_poly #() #() "Q" "lookup" in
+        "oracle".
+
+    Definition PRF_rand : val :=
+      λ:"PRF" "Q",
+        let: "lookup" := random_function (get_card_output "PRF") in
+        let: "oracle" := q_calls_poly #() #() "Q" "lookup" in
+        "oracle".
+
+  End sem.
+End sem.
+
+
+Section prf_lrel.
+  Context `{PRF_params : PRF}.
 
   Definition lrel_key {Σ} : lrel Σ := lrel_int_bounded 0 card_key.
   Definition lrel_input {Σ} : lrel Σ := lrel_int_bounded 0 card_input.
@@ -39,11 +147,10 @@ Section lrel.
 
   Definition lrel_PRF_Adv `{!approxisRGS Σ} := ((lrel_input → (lrel_option lrel_output)) → lrel_bool)%lrel.
 
-End lrel.
-
+End prf_lrel.
 
 Module LR_prf.
-  Import Ltac2 Printf.
+  Import Ltac2 (* Printf *).
   Export LR_bounded.
 
   Ltac2 Set pattern_of_lr2 as previous :=
@@ -57,18 +164,18 @@ Module LR_prf.
       end.
 
   Ltac2 prf_intro (typ : constr) xs k :=
-    printf "entering prf_intro, typ: %t" typ ;
+    (* printf "entering prf_intro, typ: %t" typ ; *)
     lazy_match! typ with
       | lrel_input =>
-          printf "found `lrel_input`, unfolding" ;
+          (* printf "found `lrel_input`, unfolding" ; *)
           let typ := eval unfold lrel_input in $typ in
             k typ xs
       | lrel_output =>
-          printf "found `lrel_output`, unfolding" ;
+          (* printf "found `lrel_output`, unfolding" ; *)
           let typ := eval unfold lrel_output in $typ in
             k typ xs
       | lrel_key =>
-          printf "found `lrel_key`, unfolding" ;
+          (* printf "found `lrel_key`, unfolding" ; *)
           let typ := eval unfold lrel_key in $typ in
             k typ xs
     | _ => None
@@ -76,15 +183,15 @@ Module LR_prf.
   Ltac2 Set Basic.lrintro_tacs as prev := fun () => FMap.add "prf" prf_intro (prev ()).
 
   Ltac2 prf_val typ k :=
-    printf "entering prf_val, typ: %t" typ ;
+    (* printf "entering prf_val, typ: %t" typ ; *)
     lazy_match! typ with
     | (lrel_car lrel_input ?v1 ?v2) =>
-        printf "found `lrel_input %t %t`, unfolding" v1 v2 ;
+        (* printf "found `lrel_input %t %t`, unfolding" v1 v2 ; *)
         (* ltac1:(iExists _ ; iPureIntro ; (intuition lia || eauto)) ; Progressed *)
         let typ := eval unfold lrel_input in $typ in
           k typ
     | (lrel_car lrel_output ?v1 ?v2) =>
-        printf "found `lrel_output %t %t`, unfolding" v1 v2 ;
+        (* printf "found `lrel_output %t %t`, unfolding" v1 v2 ; *)
         (* ltac1:(iExists _ ; iPureIntro ; (intuition lia || eauto)) ; Progressed *)
         let typ := eval unfold lrel_output in $typ in
           k typ
@@ -107,11 +214,11 @@ Export LR_prf.
 
 Section random_function.
 
-  Fact random_function_sem_typed `{!approxisRGS Σ} `{PRF} A :
-    ⊢ REL (random_function card_output)
-        << (random_function card_output) : A → lrel_input → lrel_output.
+  Fact random_function_sem_typed `{!approxisRGS Σ} {prf_params : PRF_params} :
+    ⊢ REL random_function #card_output
+        << random_function #card_output : lrel_input → lrel_output.
   Proof with (rel_pures_l ; rel_pures_r).
-    rel_arrow_val ; iIntros (??) "_".
+    (* rel_arrow_val ; (* iIntros (??) "_" *) lrintro "max". *)
     rewrite /random_function...
     rel_bind_r (init_map #()). iApply refines_init_map_r => /=... iIntros (map_r) "map_r".
     rel_bind_l (init_map #()). iApply refines_init_map_l. iIntros (map_l) "map_l" => /=...
@@ -146,7 +253,7 @@ Section random_function.
       opose proof (elem_of_map_img_2 M x y x_fresh) as hy.
       destruct (range_int y hy) as [y' [??]]. subst.
       rel_vals.
-    + rel_apply (refines_couple_UU card_output id); first auto.
+    + rel_apply (refines_couple_UU card_output id) => //.
       iIntros (y) "!> %"...
       rel_apply_r (refines_set_r with "[-map_r] [$map_r]"). iIntros "map_r"...
       rel_apply_l (refines_set_l with "[-map_l] [$map_l]"). iIntros "map_l"...
@@ -211,7 +318,7 @@ Section random_function.
 
     Lemma wp_random_function E :
       {{{ True }}}
-        random_function card_output #() @ E
+        random_function #card_output @ E
         {{{ f, RET f; is_random_function f ∅ }}}.
     Proof.
       rewrite /random_function.
@@ -223,7 +330,7 @@ Section random_function.
     Qed.
 
     Lemma spec_random_function E K:
-      ⤇ fill K (random_function card_output #()) -∗
+      ⤇ fill K (random_function #card_output) -∗
       spec_update E (∃ (f:val), ⤇ fill K f ∗ is_srandom_function f ∅).
     Proof.
       rewrite /random_function.
