theories/approxis/examples/prf_sem.v
@@ -2,25 +2,3 @@ From clutch.approxis Require Import approxis map list security_aux option.
 From clutch.approxis Require Export bounded_oracle prf.
 Set Default Proof Using "Type*".
 
-(** PRF security definitions using the variant of q_calls using semantic typing
-    instead of bounds checks. **)
-Section sem.
-
-  Context `{PRF}.
-
-  Let q_calls := q_calls_poly.
-
-  Definition PRF_real : val :=
-    λ:"Q",
-      let: "k" := keygen #() in
-      let: "lookup" := prf "k" in
-      let: "oracle" := q_calls_poly #() #() "Q" "lookup" in
-      "oracle".
-
-  Definition PRF_rand : val :=
-    λ:"Q",
-      let: "lookup" := random_function card_output #() in
-      let: "oracle" := q_calls_poly #() #() "Q" "lookup" in
-      "oracle".
-
-End sem.
